LF/Basics.lean
@@ -421,7 +421,7 @@ def nand (b1 : MyBool) (b2 : MyBool) : MyBool
 example : nand MyBool.true  MyBool.false = MyBool.true  := solution!(by rfl)
 example : nand MyBool.false MyBool.false = MyBool.true  := solution!(by rfl)
 example : nand MyBool.false MyBool.true  = MyBool.true  := solution!(by rfl)
-example : nand MyBool.true  MyBool.true  = MyBool.false := solution!(by rfl)
+theorem nand_test4 : nand MyBool.true  MyBool.true  = MyBool.false := solution!(by rfl)
 ```
 
 :::gradeTheorem 1 "nand_test4"
@@ -440,7 +440,7 @@ def and3 (b1 : MyBool) (b2 : MyBool) (b3 : MyBool) : MyBool
 example : and3 MyBool.true  MyBool.true  MyBool.true  = MyBool.true  := solution!(by rfl)
 example : and3 MyBool.false MyBool.true  MyBool.true  = MyBool.false := solution!(by rfl)
 example : and3 MyBool.true  MyBool.false MyBool.true  = MyBool.false := solution!(by rfl)
-example : and3 MyBool.true  MyBool.true  MyBool.false = MyBool.false := solution!(by rfl)
+theorem and3_test4 : and3 MyBool.true  MyBool.true  MyBool.false = MyBool.false := solution!(by rfl)
 ```
 
 :::gradeTheorem 1 "and3_test4"
@@ -592,7 +592,7 @@ theorem false_or : ∀ (b : MyBool), (MyBool.false || b) = b := by
     rfl
 ```
 
-:::gradeTheorem 1 "false_or_exercise"
+:::gradeTheorem 1 "false_or"
 :::
 ::::
 
@@ -849,11 +849,13 @@ def is_weekend (d : Day) : Bool
     | _ => false
     )
 
-example : is_weekend Day.sunday = true := solution!(by rfl)
-example : is_weekend Day.friday = false := solution!(by rfl)
+theorem is_weekend_test1 : is_weekend Day.sunday = true := solution!(by rfl)
+theorem is_weekend_test2 : is_weekend Day.friday = false := solution!(by rfl)
 ```
 
-:::gradeTheorem 1 "is_weekend"
+:::gradeTheorem "0.5" "is_weekend_test1"
+:::
+:::gradeTheorem "0.5" "is_weekend_test2"
 :::
 ::::
 
@@ -880,15 +882,21 @@ def is_inversion (c1 c2 : Color) : Bool
     | _, _ => false
     )
 
-example : is_inversion Color.black Color.white = true := solution!(by rfl)
-example : is_inversion Color.white Color.black = Bool.true := solution!(by rfl)
-example : is_inversion (Color.primary RGB.red) (Color.primary RGB.blue) = Bool.true :=
+theorem is_inversion_test1 : is_inversion Color.black Color.white = true := solution!(by rfl)
+theorem is_inversion_test2 : is_inversion Color.white Color.black = Bool.true := solution!(by rfl)
+theorem is_inversion_test3 : is_inversion (Color.primary RGB.red) (Color.primary RGB.blue) = Bool.true :=
   solution!(by rfl)
-example : is_inversion (Color.primary RGB.green) (Color.primary RGB.red) = Bool.false :=
+theorem is_inversion_test4 : is_inversion (Color.primary RGB.green) (Color.primary RGB.red) = Bool.false :=
   solution!(by rfl)
 ```
 
-:::gradeTheorem 1 "is_inversion"
+:::gradeTheorem "0.25" "is_inversion_test1"
+:::
+:::gradeTheorem "0.25" "is_inversion_test2"
+:::
+:::gradeTheorem "0.25" "is_inversion_test3"
+:::
+:::gradeTheorem "0.25" "is_inversion_test4"
 :::
 ::::
 
@@ -1857,7 +1865,15 @@ theorem two_mul_two : (two * two : Nat) = four := by
     rfl
 ```
 
-:::gradeTheorem 2 "test_mul_add"
+:::gradeTheorem "0.4" "zero_add_one"
+:::
+:::gradeTheorem "0.4" "one_add_one"
+:::
+:::gradeTheorem "0.4" "zero_mul_two"
+:::
+:::gradeTheorem "0.4" "one_mul_two"
+:::
+:::gradeTheorem "0.4" "two_mul_two"
 :::
 ::::
 
@@ -1931,7 +1947,7 @@ def blt (n m : Nat) : Bool
 
 example : blt two two = false := solution!(by rfl)
 example : blt two four = true  := solution!(by rfl)
-example : blt four two = false := solution!(by rfl)
+theorem blt_test3 : blt four two = false := solution!(by rfl)
 
 attribute [irreducible] blt ble
 ```
@@ -2322,7 +2338,7 @@ theorem or_false_true : ∀ b : Bool,
 :::
 ::::
 
-::::exercise (rating := 1) (name := "zero_nbeq_add_1")
+::::exercise (rating := 1) (name := "zero_neb_add_one")
 ```lean
 theorem zero_neb_add_one : ∀ n : Nat,
   (zero == succ n) = false := by
@@ -2332,7 +2348,7 @@ theorem zero_neb_add_one : ∀ n : Nat,
     case succ n' => rewrite [zero_succ_beq_false]; rfl
 ```
 
-:::gradeTheorem 1 "zero_nbeq_add_1"
+:::gradeTheorem 1 "zero_neb_add_one"
 :::
 ::::
 
@@ -2469,9 +2485,9 @@ def binToNat (m : Bin) : Nat
   | .b0 m' => binToNat m' * two
   | .b1 m' => binToNat m' * two + one)
 
-example : incr (.b1 .z) = .b0 (.b1 .z) := solution!(by rfl)
-example : incr (.b0 (.b1 .z)) = .b1 (.b1 .z) := solution!(by rfl)
-example : incr (.b1 (.b1 .z)) = .b0 (.b0 (.b1 .z)) := solution!(by rfl)
+theorem incr_test1 : incr (.b1 .z) = .b0 (.b1 .z) := solution!(by rfl)
+theorem incr_test2 : incr (.b0 (.b1 .z)) = .b1 (.b1 .z) := solution!(by rfl)
+theorem incr_test3 : incr (.b1 (.b1 .z)) = .b0 (.b0 (.b1 .z)) := solution!(by rfl)
 
 theorem incr_z : incr .z = .b1 .z := solution!(by rfl)
 theorem incr_b0 m : incr (.b0 m) = .b1 m := solution!(by rfl)
@@ -2490,19 +2506,18 @@ example : binToNat (.b0 (.b1 .z)) = two := solution!(by
   rewrite [binToNat_b0, binToNat_b1, binToNat_z]
   rewrite [zero_mul_two, zero_add_one, one_mul_two]
   rfl
-
 )
-example : binToNat (incr (.b1 .z)) = add one (binToNat (.b1 .z)) := solution!(by
+theorem binToNat_test1 : binToNat (incr (.b1 .z)) = add one (binToNat (.b1 .z)) := solution!(by
     rewrite [binToNat_b1, binToNat_z, incr_b1, binToNat_b0, incr_z, binToNat_b1, binToNat_z]
     rewrite [zero_mul_two, zero_add_one, one_mul_two, one_add_one]
     rfl
 )
-example : binToNat (incr (incr (.b1 .z))) = add two (binToNat (.b1 .z)) := solution!(by
+theorem binToNat_test2 : binToNat (incr (incr (.b1 .z))) = add two (binToNat (.b1 .z)) := solution!(by
   rewrite [binToNat_b1, binToNat_z, incr_b1, incr_b0, binToNat_b1, incr_z, binToNat_b1, binToNat_z]
   rewrite [zero_mul_two, zero_add_one, one_mul_two]
   rfl
 )
-example : binToNat (.b0 (.b0 (.b1 .z))) = four := solution!(by
+theorem binToNat_test3 : binToNat (.b0 (.b0 (.b1 .z))) = four := solution!(by
   rewrite [binToNat_b0, binToNat_b0, binToNat_b1, binToNat_z]
   rewrite [zero_mul_two, zero_add_one, one_mul_two, two_mul_two]
   rfl
@@ -2513,19 +2528,14 @@ attribute [irreducible] incr binToNat
 
 :::gradeTheorem "0.5" "incr_test1"
 :::
-
 :::gradeTheorem "0.5" "incr_test2"
 :::
-
 :::gradeTheorem "0.5" "incr_test3"
 :::
-
 :::gradeTheorem "0.5" "binToNat_test1"
 :::
-
 :::gradeTheorem "0.5" "binToNat_test2"
 :::
-
 :::gradeTheorem "0.5" "binToNat_test3"
 :::
 ::::
@@ -2783,21 +2793,18 @@ def gradeComparison (g1 g2 : Grade) : Comparison
   | eq => modifierComparison g1.modifier g2.modifier
   | gt => gt)
 
-example : gradeComparison ⟨A, minus⟩ ⟨B, plus⟩ = gt := solution!(by rfl)
-example : gradeComparison ⟨A, minus⟩ ⟨A, plus⟩ = lt := solution!(by rfl)
-example : gradeComparison ⟨F, plus⟩ ⟨F, plus⟩ = eq := solution!(by rfl)
-example : gradeComparison ⟨B, minus⟩ ⟨C, plus⟩ = gt := solution!(by rfl)
+theorem gradeComparison_test1 : gradeComparison ⟨A, minus⟩ ⟨B, plus⟩ = gt := solution!(by rfl)
+theorem gradeComparison_test2 : gradeComparison ⟨A, minus⟩ ⟨A, plus⟩ = lt := solution!(by rfl)
+theorem gradeComparison_test3 : gradeComparison ⟨F, plus⟩ ⟨F, plus⟩ = eq := solution!(by rfl)
+theorem gradeComparison_test4 : gradeComparison ⟨B, minus⟩ ⟨C, plus⟩ = gt := solution!(by rfl)
 ```
 
 :::gradeTheorem "0.5" "gradeComparison_test1"
 :::
-
 :::gradeTheorem "0.5" "gradeComparison_test2"
 :::
-
 :::gradeTheorem "0.5" "gradeComparison_test3"
 :::
-
 :::gradeTheorem "0.5" "gradeComparison_test4"
 :::
 ::::
@@ -2860,21 +2867,19 @@ def lowerGrade (g : Grade) : Grade
   | ⟨F, minus⟩ => ⟨F, minus⟩
   | ⟨l, minus⟩ => ⟨lowerLetter l, plus⟩)
 
-example : lowerGrade ⟨A, plus⟩ = ⟨A, natural⟩ := solution!(by rfl)
+theorem lowerGrade_A_plus : lowerGrade ⟨A, plus⟩ = ⟨A, natural⟩ := solution!(by rfl)
 example : lowerGrade ⟨A, natural⟩ = ⟨A, minus⟩ := solution!(by rfl)
 example : lowerGrade ⟨A, minus⟩ = ⟨B, plus⟩ := solution!(by rfl)
 example : lowerGrade ⟨B, plus⟩ = ⟨B, natural⟩ := solution!(by rfl)
 example : lowerGrade ⟨F, natural⟩ = ⟨F, minus⟩ := solution!(by rfl)
 example : lowerGrade (lowerGrade ⟨B, minus⟩) = ⟨C, natural⟩ := solution!(by rfl)
 example : lowerGrade (lowerGrade (lowerGrade ⟨B, minus⟩)) = ⟨C, minus⟩ := solution!(by rfl)
-
-theorem lowerGrade_F_Minus : lowerGrade ⟨F, minus⟩ = ⟨F, minus⟩ := solution!(by rfl)
+theorem lowerGrade_F_minus : lowerGrade ⟨F, minus⟩ = ⟨F, minus⟩ := solution!(by rfl)
 ```
 
-:::gradeTheorem "0.25" "lowerGrade_A_Plus"
+:::gradeTheorem "0.25" "lowerGrade_A_plus"
 :::
-
-:::gradeTheorem "0.25" "lowerGrade_F_Minus"
+:::gradeTheorem "0.25" "lowerGrade_F_minus"
 :::
 ::::
 
@@ -2908,7 +2913,7 @@ theorem lowerGrade_lowers : ∀ g : Grade,
       contradiction
     | ⟨l, minus⟩ =>
       cases l
-      case F => rewrite [lowerGrade_F_Minus]; exact h
+      case F => rewrite [lowerGrade_F_minus]; exact h
       all_goals rfl
 ```
 
@@ -2918,6 +2923,14 @@ that you might need the `contradiction` tactic here instead,
 or some other reasoning that's not accomplishable
 with the tactics we've introduced so far. Can you make this
 proof work with only `rw`, `rfl`, `exact`, etc?
+
+Niklas Halonen (xhalo32): We need to teach how to prove a goal that looks like `natural ≠ minus` for example.
+One could write `injection x` for example:
+```lean
+example : natural ≠ minus := by
+  intro x
+  injection x
+```
 :::
 
 :::gradeTheorem 3 "lowerGrade_lowers"
